Soundness of eval: QED

core_c_trivial_bigstep.v
@@ -10,29 +10,148 @@ Notation store := (list (option Z)).
 
 Inductive mem_stack `{Env K} (Γ : env K) (Δ : memenv K): stack K -> store -> mem K -> Prop :=
 | mem_stack_empty m:
+  ✓ Γ ->
+  ✓{Γ} Δ ->
+  ✓{Γ, Δ} m ->
   mem_stack Γ Δ [] [] m
 | mem_stack_alloc o mv m ρ st m':
+  ✓ Γ ->
+  ✓{Γ} Δ ->
+  index_alive Δ o ->
   mem_singleton Γ Δ (addr_top o sintT%T) false perm_full
     (match mv with None => indetV sintT%BT | Some z => intV{sintT} z end)
     sintT%T m ->
   mem_stack Γ Δ ρ st m' ->
-  m ⊥ m' ->
+  ⊥[m; m'] ->
   mem_stack Γ Δ ((o, sintT%T)::ρ) (mv::st) (m ∪ m')
 .
+
+Lemma mem_stack_valid `{EnvSpec K} Γ Δ ρ st m:
+  mem_stack Γ Δ ρ st m ->
+  ✓{Γ, Δ} m.
+induction 1.
+- assumption.
+- apply cmap_union_valid_2.
+  * apply sep_disjoint_list_double; assumption.
+  * apply mem_singleton_valid with (4:=H4); try assumption.
+    discriminate.
+  * assumption.
+Qed.
+
+Lemma mem_stack_lookup_stack `{Env K} Γ Δ ρ st m i mv:
+  mem_stack Γ Δ ρ st m ->
+  st !! i = Some mv ->
+  exists o, ρ !! i = Some (o, sintT%T).
+intro.
+revert i mv.
+induction H0.
+- intros.
+  discriminate.
+- intros.
+  destruct i.
+  + exists o. reflexivity.
+  + simpl in H6.
+    simpl.
+    apply IHmem_stack with (1:=H6).
+Qed.
+
+Lemma mem_stack_lookup_mem `{EnvSpec K} Γ Δ ρ st m i v o:
+  mem_stack Γ Δ ρ st m ->
+  st !! i = Some (Some v) ->
+  ρ !! i = Some (o, sintT%T) ->
+  m !!{Γ} addr_top o sintT%T = Some (intV{sintT} v).
+intro.
+revert i v o.
+induction H1; intros. {
+  discriminate.
+}
+destruct i; simpl in *.
+- injection H7; clear H7; intros; subst.
+  injection H8; clear H8; intros; subst.
+  eapply mem_lookup_subseteq with (m1:=m).
+  + assumption.
+  + apply mem_singleton_valid with (4:=H4).
+    * assumption.
+    * assumption.
+    * discriminate.
+    * apply H3.
+  + apply sep_union_subseteq_l.
+    assumption.
+  + apply mem_lookup_singleton with (3:=H4).
+    * assumption.
+    * rewrite perm_kind_full.
+      reflexivity.
+- eapply mem_lookup_subseteq with (m1:=m').
+  + assumption.
+  + apply mem_stack_valid with (1:=H5).
+  + apply sep_union_subseteq_r.
+    assumption.
+  + apply IHmem_stack with (1:=H7) (2:=H8).
+Qed.
+
+Lemma mem_stack_forced `{EnvSpec K} Γ Δ ρ st m i v o:
+  mem_stack Γ Δ ρ st m ->
+  st !! i = Some (Some v) ->
+  ρ !! i = Some (o, sintT%T) ->
+  mem_forced Γ (addr_top o sintT%T) m.
+intro.
+revert i v o.
+induction H1; intros. {
+  discriminate.
+}
+destruct i; simpl in *.
+- injection H7; clear H7; intros; subst.
+  injection H8; clear H8; intros; subst.
+  eapply mem_forced_subseteq with (m1:=m); try eassumption.
+  + apply mem_singleton_valid with (4:=H4); try assumption.
+    discriminate.
+  + apply sep_union_subseteq_l. assumption.
+  + apply mem_singleton_forced with (3:=H4).
+    * assumption.
+    * rewrite perm_kind_full.
+      reflexivity.
+  + rewrite mem_lookup_singleton with (3:=H4).
+    * unfold is_Some.
+      eexists. reflexivity.
+    * assumption.
+    * rewrite perm_kind_full. reflexivity.
+- eapply mem_forced_subseteq with (m1:=m').
+  + assumption.
+  + apply mem_stack_valid with (1:=H5).
+  + apply sep_union_subseteq_r.
+    assumption.
+  + eapply IHmem_stack; eassumption.
+  + rewrite mem_stack_lookup_mem with (1:=H5) (2:=H7) (3:=H8).
+    eexists; reflexivity.
+Qed.
 
 Inductive eval `{Env K}: store -> expr K -> Z -> Prop :=
 | eval_lit st z:
   eval st (# intV{sintT} z) z
-| eval_var st i z:
+| eval_load_var st i z:
   st !! i = Some (Some z) ->
   eval st (load (var i)) z
 .
 
-Lemma eval_sound `{Env K} (Γ: env K) st e z ρ m:
+Lemma eval_sound `{EnvSpec K} (Γ: env K) st e z ρ m:
   eval st e z ->
   mem_stack Γ '{m} ρ st m ->
   ⟦ e ⟧ Γ ρ m = Some (inr (intV{sintT} z)).
-Admitted.
+intros.
+destruct H1.
+- (* eval_lit *)
+  reflexivity.
+- (* eval_load_var *)
+  simpl.
+  pose proof (mem_stack_lookup_stack _ _ _ _ _ _ _ H2 H1).
+  destruct H3 as [o Ho].
+  rewrite Ho.
+  simpl.
+  rewrite option_guard_True.
+  + rewrite mem_stack_lookup_mem with (1:=H2) (2:=H1) (3:=Ho).
+    reflexivity.
+  + apply mem_stack_forced with (1:=H2) (2:=H1) (3:=Ho).
+Qed.
 
 Inductive outcome := onormal(s: store) | oreturn(z: Z).
 
